@prefix alg:    <http://www.w3id.org/dice-research/ontologies/algorithm/2023/06/> .
@prefix dcat:   <http://www.w3.org/ns/dcat#> .
@prefix enexa:  <http://w3id.org/dice-research/enexa/ontology#> .
@prefix hobbit: <http://w3id.org/hobbit/vocab#> .
@prefix owl:    <http://www.w3.org/2002/07/owl#> .
@prefix prov:   <http://www.w3.org/ns/prov#> .
@prefix rdf:    <http://www.w3.org/1999/02/22-rdf-syntax-ns#> .
@prefix rdfs:   <http://www.w3.org/2000/01/rdf-schema#> .

<http://w3id.org/dice-research/enexa/module/transform/0.0.1> a enexa:Module ;
	rdfs:label "ENEXA Transformation Module"@en ;
	rdfs:comment "This module allows the transformation and concatenation of RDF datasets."@en ;
	hobbit:image <urn:container:docker:image:docker.io/library/dice-group/enexa-transform:0.0.1> ;
	alg:parameter <http://w3id.org/dice-research/enexa/module/transform/parameter/input> ;
	alg:parameter <http://w3id.org/dice-research/enexa/module/transform/parameter/outputMediaType> ;
	alg:produces <http://w3id.org/dice-research/enexa/module/transform/result/output> .

<http://w3id.org/dice-research/enexa/module/transform/parameter/input> a alg:Parameter ;
	rdfs:label "Input dataset" ;
	rdfs:comment "An RDF dataset that is used as input for the transformation." .	

<http://w3id.org/dice-research/enexa/module/transform/parameter/outputMediaType> a alg:Parameter ;
	rdfs:label "Output format" ;
	rdfs:comment "The format of the output dataset." ;	
	rdfs:range <http://w3id.org/dice-research/enexa/module/transform/StreamableRDFSerialization> .

<http://w3id.org/dice-research/enexa/module/transform/result/output> a alg:Result ;
	rdfs:label "Output dataset" ;
	rdfs:comment "The output dataset that is created as result of the transformation." ;	
	rdfs:range prov:Entity .

<http://w3id.org/dice-research/enexa/module/transform/StreamableRDFSerialization> a owl:Class ;
	rdfs:label "stream-able RDF serializations" ;
	rdfs:comment "The class of RDF serializations that can be streamed and, hence, are supported as output format by the ENEXA transformator module." .

<https://www.iana.org/assignments/media-types/application/n-quads> a <http://w3id.org/dice-research/enexa/module/transform/StreamableRDFSerialization> ;
	rdfs:label "N-Quads" ;
	rdfs:comment "N-Quads is a line-based, plain text format for encoding an RDF dataset." ;
	rdfs:isDefinedBy <https://www.w3.org/TR/n-quads/> .
	
<https://www.iana.org/assignments/media-types/application/n-triples> a <http://w3id.org/dice-research/enexa/module/transform/StreamableRDFSerialization> ;
	rdfs:label "N-Triples" ;
	rdfs:comment "N-Triples is a line-based, plain text format for encoding an RDF graph." ;
	rdfs:isDefinedBy <https://www.w3.org/TR/n-triples/> .

<https://www.iana.org/assignments/media-types/application/trig> a <http://w3id.org/dice-research/enexa/module/transform/StreamableRDFSerialization> ;
	rdfs:label "TriG" ;
	rdfs:comment "TriG is a concrete syntax for RDF as defined in the RDF Concepts and Abstract Syntax document, and an extension of Turtle to support representing a complete RDF Dataset." ;
	rdfs:isDefinedBy <https://www.w3.org/TR/trig/> .

<https://www.iana.org/assignments/media-types/text/turtle> a <http://w3id.org/dice-research/enexa/module/transform/StreamableRDFSerialization> ;
	rdfs:label "Turtle" ;
	rdfs:comment "The terse RDF Triple Language (Turtle) is a concrete syntax for RDF as defined in the RDF Concepts and Abstract Syntax W3C Recommendation." ;
	rdfs:isDefinedBy <https://www.w3.org/TeamSubmission/turtle/> .

@prefix alg:    <http://www.w3id.org/dice-research/ontologies/algorithm/2023/06/> .
@prefix dcat:   <http://www.w3.org/ns/dcat#> .
@prefix enexa:  <http://w3id.org/dice-research/enexa/ontology#> .
@prefix hobbit: <http://w3id.org/hobbit/vocab#> .
@prefix owl:    <http://www.w3.org/2002/07/owl#> .
@prefix prov:   <http://www.w3.org/ns/prov#> .
@prefix rdf:    <http://www.w3.org/1999/02/22-rdf-syntax-ns#> .
@prefix rdfs:   <http://www.w3.org/2000/01/rdf-schema#> .

<http://w3id.org/dice-research/enexa/module/transform/0.0.1> a enexa:Module ;
	rdfs:label "ENEXA Transformation Module"@en ;
	rdfs:comment "This module allows the transformation and concatenation of RDF datasets."@en ;
	hobbit:image <urn:container:docker:image:hub.cs.upb.de/enexa/enexa-transform-module:0.0.1> ;
	alg:parameter <http://w3id.org/dice-research/enexa/module/transform/parameter/input> ;
	alg:parameter <http://w3id.org/dice-research/enexa/module/transform/parameter/outputMediaType> ;
	alg:produces <http://w3id.org/dice-research/enexa/module/transform/result/output> .

<http://w3id.org/dice-research/enexa/module/transform/parameter/input> a alg:Parameter ;
	rdfs:label "Input dataset" ;
	rdfs:comment "An RDF dataset that is used as input for the transformation." .	

<http://w3id.org/dice-research/enexa/module/transform/parameter/outputMediaType> a alg:Parameter ;
	rdfs:label "Output format" ;
	rdfs:comment "The format of the output dataset." ;	
	rdfs:range <http://w3id.org/dice-research/enexa/module/transform/StreamableRDFSerialization> .

<http://w3id.org/dice-research/enexa/module/transform/result/output> a alg:Result ;
	rdfs:label "Output dataset" ;
	rdfs:comment "The output dataset that is created as result of the transformation." ;	
	rdfs:range prov:Entity .

<http://w3id.org/dice-research/enexa/module/transform/StreamableRDFSerialization> a owl:Class ;
	rdfs:label "stream-able RDF serializations" ;
	rdfs:comment "The class of RDF serializations that can be streamed and, hence, are supported as output format by the ENEXA transformator module." .

<https://www.iana.org/assignments/media-types/application/n-quads> a <http://w3id.org/dice-research/enexa/module/transform/StreamableRDFSerialization> ;
	rdfs:label "N-Quads" ;
	rdfs:comment "N-Quads is a line-based, plain text format for encoding an RDF dataset." ;
	rdfs:isDefinedBy <https://www.w3.org/TR/n-quads/> .
	
<https://www.iana.org/assignments/media-types/application/n-triples> a <http://w3id.org/dice-research/enexa/module/transform/StreamableRDFSerialization> ;
	rdfs:label "N-Triples" ;
	rdfs:comment "N-Triples is a line-based, plain text format for encoding an RDF graph." ;
	rdfs:isDefinedBy <https://www.w3.org/TR/n-triples/> .

<https://www.iana.org/assignments/media-types/application/trig> a <http://w3id.org/dice-research/enexa/module/transform/StreamableRDFSerialization> ;
	rdfs:label "TriG" ;
	rdfs:comment "TriG is a concrete syntax for RDF as defined in the RDF Concepts and Abstract Syntax document, and an extension of Turtle to support representing a complete RDF Dataset." ;
	rdfs:isDefinedBy <https://www.w3.org/TR/trig/> .

<https://www.iana.org/assignments/media-types/text/turtle> a <http://w3id.org/dice-research/enexa/module/transform/StreamableRDFSerialization> ;
	rdfs:label "Turtle" ;
	rdfs:comment "The terse RDF Triple Language (Turtle) is a concrete syntax for RDF as defined in the RDF Concepts and Abstract Syntax W3C Recommendation." ;
	rdfs:isDefinedBy <https://www.w3.org/TeamSubmission/turtle/> .

